compiler/backend/stack_to_labScript.sml
@@ -14,7 +14,7 @@ val _ = patternMatchesLib.ENABLE_PMATCH_CASES();
 val _ = temp_overload_on ("Asm",``λa. Asm (Asmi a)``);
 
 val compile_jump_def = Define `
-  (compile_jump (INL n) = LabAsm (Jump (Lab n 0)) 0w [] 0) /\
+  (compile_jump (INL n) = LabAsm (Jump (Lab n.fname 0)) 0w [] 0) /\
   (compile_jump (INR r) = Asm (JumpReg r) [] 0)`;
 
 val negate_def = Define `
@@ -46,48 +46,48 @@ local val flatten_quotation = `
         let (ys,nr2,m) = flatten p2 n m in
           if (p1 = Skip) /\ (p2 = Skip) then (List [],F,m)
           else if p1 = Skip then
-            (List [LabAsm (JumpCmp c r ri (Lab n m)) 0w [] 0] ++ ys ++
-             List [Label n m 0],F,m+1)
+            (List [LabAsm (JumpCmp c r ri (Lab n.fname m)) 0w [] 0] ++ ys ++
+             List [Label n.fname m 0],F,m+1)
           else if p2 = Skip then
-            (List [LabAsm (JumpCmp (negate c) r ri (Lab n m)) 0w [] 0] ++ xs ++
-             List [Label n m 0],F,m+1)
+            (List [LabAsm (JumpCmp (negate c) r ri (Lab n.fname m)) 0w [] 0] ++ xs ++
+             List [Label n.fname m 0],F,m+1)
           else if nr1 then
-            (List [LabAsm (JumpCmp (negate c) r ri (Lab n m)) 0w [] 0] ++ xs ++
-             List [Label n m 0] ++ ys,nr2,m+1)
+            (List [LabAsm (JumpCmp (negate c) r ri (Lab n.fname m)) 0w [] 0] ++ xs ++
+             List [Label n.fname m 0] ++ ys,nr2,m+1)
           else if nr2 then
-            (List [LabAsm (JumpCmp c r ri (Lab n m)) 0w [] 0] ++ ys ++
-             List [Label n m 0] ++ xs,nr1,m+1)
+            (List [LabAsm (JumpCmp c r ri (Lab n.fname m)) 0w [] 0] ++ ys ++
+             List [Label n.fname m 0] ++ xs,nr1,m+1)
           else
-            (List [LabAsm (JumpCmp c r ri (Lab n m)) 0w [] 0] ++ ys ++
-             List [LabAsm (Jump (Lab n (m+1))) 0w [] 0; Label n m 0] ++ xs ++
-             List [Label n (m+1) 0],nr1 ∧ nr2,m+2)
+            (List [LabAsm (JumpCmp c r ri (Lab n.fname m)) 0w [] 0] ++ ys ++
+             List [LabAsm (Jump (Lab n.fname (m+1))) 0w [] 0; Label n.fname m 0] ++ xs ++
+             List [Label n.fname (m+1) 0],nr1 ∧ nr2,m+2)
     | While c r ri p1 =>
         let (xs,_,m) = flatten p1 n m in
-          (List [Label n m 0; LabAsm (JumpCmp (negate c) r ri (Lab n (m+1))) 0w [] 0] ++
-           xs ++ List [LabAsm (Jump (Lab n m)) 0w [] 0; Label n (m+1) 0],F,m+2)
+          (List [Label n.fname m 0; LabAsm (JumpCmp (negate c) r ri (Lab n.fname (m+1))) 0w [] 0] ++
+           xs ++ List [LabAsm (Jump (Lab n.fname m)) 0w [] 0; Label n.fname (m+1) 0],F,m+2)
     | Raise r => (List [Asm (JumpReg r) [] 0],T,m)
     | Return r _ => (List [Asm (JumpReg r) [] 0],T,m)
-    | Call NONE dest handler => (List [compile_jump dest],T,m)
-    | Call (SOME (p1,lr,l1,l2)) dest handler =>
+    | stackLang$Call NONE dest handler => (List [compile_jump dest],T,m)
+    | stackLang$Call (SOME (p1,lr,l1,l2)) dest handler =>
         let (xs,nr1,m) = flatten p1 n m in
-        let prefix = List [LabAsm (LocValue lr (Lab l1 l2)) 0w [] 0;
-                 compile_jump dest; Label l1 l2 0] ++ xs in
+        let prefix = List [LabAsm (LocValue lr (Lab l1.fname l2)) 0w [] 0;
+                 compile_jump dest; Label l1.fname l2 0] ++ xs in
         (dtcase handler of
         | NONE => (prefix, nr1, m)
         | SOME (p2,k1,k2) =>
             let (ys,nr2,m) = flatten p2 n m in
-              (prefix ++ (List [LabAsm (Jump (Lab n m)) 0w [] 0; Label k1 k2 0] ++
-              ys ++ List [Label n m 0]), nr1 ∧ nr2, m+1))
+              (prefix ++ (List [LabAsm (Jump (Lab n.fname m)) 0w [] 0; Label k1.fname k2 0] ++
+              ys ++ List [Label n.fname m 0]), nr1 ∧ nr2, m+1))
     | JumpLower r1 r2 target =>
         (List [LabAsm (JumpCmp Lower r1 (Reg r2) (Lab target 0)) 0w [] 0],F,m)
-    | FFI ffi_index _ _ _ _ lr => (List [LabAsm (LocValue lr (Lab n m)) 0w [] 0;
+    | FFI ffi_index _ _ _ _ lr => (List [LabAsm (LocValue lr (Lab n.fname m)) 0w [] 0;
                                          LabAsm (CallFFI ffi_index) 0w [] 0;
-                                         Label n m 0],F,m+1)
-    | LocValue i l1 l2 => (List [LabAsm (LocValue i (Lab l1 l2)) 0w [] 0],F,m)
+                                         Label n.fname m 0],F,m+1)
+    | LocValue i l1 l2 => (List [LabAsm (LocValue i (Lab l1.fname l2)) 0w [] 0],F,m)
     | Install _ _ _ _ ret =>
-      (List [LabAsm (LocValue ret (Lab n m)) 0w [] 0;
+      (List [LabAsm (LocValue ret (Lab n.fname m)) 0w [] 0;
       LabAsm Install 0w [] 0;
-      Label n m 0],F,m+1)
+      Label n.fname m 0],F,m+1)
     | CodeBufferWrite r1 r2 =>
       (List [Asm (Cbw r1 r2) [] 0],F,m)
     | _  => (List [],F,m)`
@@ -108,7 +108,7 @@ end
 val prog_to_section_def = Define `
   prog_to_section (n,p) =
     let (lines,_,m) = (flatten p n (next_lab p 1)) in
-      Section n (append (Append lines (List [Label n m 0])))`
+      Section n.fname (append (Append lines (List [Label n.fname m 0])))`
 
 val is_gen_gc_def = Define `
   (is_gen_gc (Generational l) = T) /\
