compiler/backend/clos_callScript.sml
@@ -103,13 +103,14 @@ val EL_MEM_LEMMA = Q.prove(
   Induct \\ fs [] \\ REPEAT STRIP_TAC \\ Cases_on `i` \\ fs []);
 
 val insert_each_def = Define `
-  (insert_each p 0 g = g) /\
-  (insert_each p (SUC n) (g1,g2) = insert_each (p+2) n (insert p () g1,g2))`
+  (insert_each loc 0 g = g) /\
+  (insert_each loc (SUC n) (g1,g2) = insert_each (FNA ((+) 2) loc) n
+    (insert_fn loc () g1,g2))`
 
 val code_list_def = Define `
   (code_list loc [] g = g) /\
   (code_list loc ((n,p)::xs) (g1,g2) =
-     code_list (loc+2n) xs (g1,(loc+1,n,p)::g2))`
+     code_list (FNA ((+) 2) loc) xs (g1,(FNA ((+) 1) loc,n,p)::g2))`
 
 val GENLIST_Var_def = Define `
   GENLIST_Var t i n =
@@ -119,12 +120,16 @@ val GENLIST_Var_def = Define `
 val calls_list_def = Define `
   (calls_list t i loc [] = []) /\
   (calls_list t i loc ((n,_)::xs) =
-     (n,Call (t§i§0) 0 (loc+1) (GENLIST_Var (t§i) 1 n))::
-          calls_list t (i+1) (loc+2n) xs)`;
+     (n,Call (t§i§0) 0 (FNA ((+) 1) loc) (GENLIST_Var (t§i) 1 n))::
+          calls_list t (i+1) (FNA ((+) 2) loc) xs)`;
 
 val exp3_size_MAP_SND = Q.prove(
   `!fns. exp3_size (MAP SND fns) <= exp1_size fns`,
   Induct \\ fs [exp_size_def,FORALL_PROD]);
+
+(* An irrelevant function identifier. *)
+val irrelevant_fname_def = Define `
+  irrelevant_fname = Function_Name 0xDEDBEEF`;
 
 val calls_def = tDefine "calls" `
   (calls [] g = ([],g)) /\
@@ -171,28 +176,30 @@ val calls_def = tDefine "calls" `
      let (es,g) = calls xs g in
      let (e1,g) = calls [x] g in
      let e1 = HD e1 in
-     let loc = (case loc_opt of SOME loc => loc | NONE => 0) in
-       if IS_SOME loc_opt /\ IS_SOME (lookup loc (FST g)) then
-         if pure x then ([Call t (LENGTH es) (loc+1) es],g) else
+     let loc = (case loc_opt of SOME loc => loc | NONE => irrelevant_fname) in
+     let nloc = FNA ((+) 1) loc in
+       if IS_SOME loc_opt /\ IS_SOME (lookup_fn loc (FST g)) then
+         if pure x then ([Call t (LENGTH es) nloc es],g) else
            ([Let (t§0) (SNOC e1 es)
-              (Call (t§1) (LENGTH es) (loc+1) (GENLIST_Var t 2 (LENGTH es)))],g)
+              (Call (t§1) (LENGTH es) nloc (GENLIST_Var t 2 (LENGTH es)))],g)
        else ([App t loc_opt e1 es],g)) /\
   (calls [Fn t loc_opt ws num_args x1] g =
      (* loc_opt ought to be SOME loc, with loc being EVEN *)
-     let loc = (case loc_opt of SOME loc => loc | NONE => 0) in
+     let loc = (case loc_opt of SOME loc => loc | NONE => irrelevant_fname) in
+     let nloc = FNA ((+) 1) loc in
      let new_g = insert_each loc 1 g in
      let (e1,new_g) = calls [x1] new_g in
-     let new_g = (FST new_g,(loc+1,num_args,HD e1)::SND new_g) in
+     let new_g = (FST new_g,(nloc,num_args,HD e1)::SND new_g) in
        (* Closedness is checked on the transformed program because
           the calls function can sometimes remove free variables. *)
        if closed (Fn t loc_opt ws num_args (HD e1)) then
          ([Fn (t§0) loc_opt ws num_args
-             (Call (t§0§0) 0 (loc+1) (GENLIST_Var (t§0) 1 num_args))],new_g)
+             (Call (t§0§0) 0 (nloc) (GENLIST_Var (t§0) 1 num_args))],new_g)
        else
          let (e1,g) = calls [x1] g in
            ([Fn t loc_opt ws num_args (HD e1)],g)) /\
   (calls [Letrec t loc_opt ws fns x1] g =
-     let loc = (case loc_opt of SOME loc => loc | NONE => 0) in
+     let loc = (case loc_opt of SOME loc => loc | NONE => irrelevant_fname) in
      let new_g = insert_each loc (LENGTH fns) g in
      let (fns1,new_g) = calls (MAP SND fns) new_g in
        if EVERY2 (\(n,_) p. closed (Fn t NONE NONE n p)) fns fns1 then
@@ -239,9 +246,9 @@ Theorem compile_nil
 
 val selftest = let
   (* example code *)
-  val f = ``Fn None (SOME 800) NONE 1 (Op None Add [Var None 0; Op None (Const 1) []])``
-  val g = ``Fn None (SOME 900) NONE 1 (App None (SOME 800) (Var None 1) [Var None 0])``
-  val f_g_5 = ``App None (SOME 800) (Var None 1) [App None (SOME 900) (Var None 0) [Op None (Const 5) []]]``
+  val f = ``Fn None (SOMEF 800) NONE 1 (Op None Add [Var None 0; Op None (Const 1) []])``
+  val g = ``Fn None (SOMEF 900) NONE 1 (App None (SOMEF 800) (Var None 1) [Var None 0])``
+  val f_g_5 = ``App None (SOMEF 800) (Var None 1) [App None (SOMEF 900) (Var None 0) [Op None (Const 5) []]]``
   val let_let = ``[Let None [^f] (Let None [^g] ^f_g_5)]``
   (* compiler evaluation *)
   val tm = EVAL ``compile T ^let_let`` |> concl
