compiler/backend/clos_numberScript.sml
@@ -40,10 +40,10 @@ val renumber_code_locs_def = tDefine "renumber_code_locs" `
        (n,App t NONE x1 x2)) /\
   (renumber_code_locs n (Fn t loc vs num_args x1) =
      let (n,x1) = renumber_code_locs n x1 in
-       (n+2,Fn t (SOME n) vs num_args x1)) /\
+       (FNA ((+) 2) n,Fn t (SOME n) vs num_args x1)) /\
   (renumber_code_locs n (Letrec t loc vs fns x1) =
      let (m,fns') = renumber_code_locs_list n (MAP SND fns) in
-     let (n,x1) = renumber_code_locs (m+2*LENGTH fns') x1 in
+     let (n,x1) = renumber_code_locs (FNA ((+) (2*LENGTH fns')) m) x1 in
        (n,Letrec t (SOME m) vs (ZIP (MAP FST fns, fns')) x1)) /\
   (renumber_code_locs n (Handle t x1 x2) =
      let (n,x1) = renumber_code_locs n x1 in
@@ -65,7 +65,7 @@ val renumber_code_locs_ind = theorem"renumber_code_locs_ind";
 
 Theorem renumber_code_locs_length
   `(∀x y. LENGTH (SND (renumber_code_locs_list x y)) = LENGTH y) ∧
-    (∀(x:num)(y:closLang$exp). T)`
+    (∀(x:fname)(y:closLang$exp). T)`
     (ho_match_mp_tac renumber_code_locs_ind >>
     simp[renumber_code_locs_def,UNCURRY] >> rw[] >>
     METIS_TAC[PAIR,FST,SND]);
