compiler/backend/word_elimScript.sml
@@ -13,18 +13,18 @@ val _ = new_theory "word_elim";
 
 
 val find_word_loc_def = Define `
-    (find_word_loc (name:num, _, _) = name)
+    (find_word_loc (name:fname, _, _) = name)
 `
 
 val find_word_ref_def = Define `
     (find_word_ref (MustTerminate p) = find_word_ref p) ∧
     (find_word_ref (Call ret target _ handler) = union
-        (case target of | NONE => LN | SOME n => (insert n () LN))
+        (case target of | NONE => LN | SOME n => (insert_fn n () LN))
             (union
                 (case ret of
                     | NONE => LN
                     | SOME (_,_,ret_handler,l1,_) =>
-                        insert l1 () (find_word_ref (ret_handler)))
+                        insert_fn l1 () (find_word_ref (ret_handler)))
                 (case handler of
                     | NONE => LN
                     | SOME (_,ex_handler,_,_) => find_word_ref (ex_handler)))
@@ -32,7 +32,7 @@ val find_word_ref_def = Define `
     (find_word_ref (Seq p1 p2) = union (find_word_ref p1) (find_word_ref p2)) ∧
     (find_word_ref (If _ _ _ p1 p2) =
         union (find_word_ref p1) (find_word_ref p2)) ∧
-    (find_word_ref (LocValue _ n) = insert n () LN) ∧
+    (find_word_ref (LocValue _ n) = insert_fn n () LN) ∧
     (find_word_ref _ = LN)
 `
 
